<?xml version="1.0"?>


<!DOCTYPE rdf:RDF [
    <!ENTITY sioc "http://rdfs.org/sioc/ns#" >
    <!ENTITY dcterms "http://purl.org/dc/terms/" >
    <!ENTITY owl "http://www.w3.org/2002/07/owl#" >
    <!ENTITY dc "http://purl.org/dc/elements/1.1/" >
    <!ENTITY xsd "http://www.w3.org/2001/XMLSchema#" >
    <!ENTITY skos "http://www.w3.org/2004/02/skos/core#" >
    <!ENTITY rdfs "http://www.w3.org/2000/01/rdf-schema#" >
    <!ENTITY prv "http://lod-dk/ontologies/ProvisionModel#" >
    <!ENTITY cdm "http://publications.europa.eu/ontology/cdm#" >
    <!ENTITY rdf "http://www.w3.org/1999/02/22-rdf-syntax-ns#" >
    <!ENTITY lod "http://lod-dk/ontologies/LOD_Epartcipation#" >
    <!ENTITY at "http://publications.europa.eu/resource/authority#" >
]>


<rdf:RDF xmlns="http://lod-dk/ontologies/LOD_Eparticipation#"
     xml:base="http://lod-dk/ontologies/LOD_Eparticipation"
     xmlns:dc="http://purl.org/dc/elements/1.1/"
     xmlns:prv="http://lod-dk/ontologies/ProvisionModel#"
     xmlns:at="http://publications.europa.eu/resource/authority#"
     xmlns:lod="http://lod-dk/ontologies/LOD_Epartcipation#"
     xmlns:dcterms="http://purl.org/dc/terms/"
     xmlns:sioc="http://rdfs.org/sioc/ns#"
     xmlns:rdfs="http://www.w3.org/2000/01/rdf-schema#"
     xmlns:cdm="http://publications.europa.eu/ontology/cdm#"
     xmlns:owl="http://www.w3.org/2002/07/owl#"
     xmlns:xsd="http://www.w3.org/2001/XMLSchema#"
     xmlns:rdf="http://www.w3.org/1999/02/22-rdf-syntax-ns#"
     xmlns:skos="http://www.w3.org/2004/02/skos/core#">
    <owl:Ontology rdf:about="http://lod-dk/ontologies/LOD_Eparticipation#">
        <owl:versionInfo>Revision: 1.02</owl:versionInfo>
        <dc:creator>FRANCESCONI Enrico and BATOUCHE Brahim </dc:creator>
        <dc:date>2016-08-24</dc:date>
        <dcterms:title xml:lang="en">Electronic Partcipation Model (EPM) Core Ontology Namespace</dcterms:title>
        <rdfs:comment xml:lang="en">The Electronic Partcipation Model (EPM) of the Publications Office is an ontology for describing the information in online communities. 
This information can be used to export information from online communities and to link them together with a legal resource. The scope of the application areas that EPM can be used for includes (and is not limited to) weblogs, 
message boards, mailing lists and chat channels. The concepts of this ontology are already specified in SIOC, CDM, FOAF, and SKOS.</rdfs:comment>
        <dc:language>en</dc:language>
        <dc:description rdf:resource="http://lod-dk:8000/ontologies/lodep_ontology.jpg"/>
        <rdfs:seeAlso rdf:resource="http://rdfs.org/sioc/spec"/>
    </owl:Ontology>
    


    <!-- 
    ///////////////////////////////////////////////////////////////////////////////////////
    //
    // Annotation properties
    //
    ///////////////////////////////////////////////////////////////////////////////////////
     -->

    


    <!-- http://lod-dk/ontologies/LOD_Epartcipation#directory_code -->

    <owl:AnnotationProperty rdf:about="&lod;directory_code">
        <rdfs:comment xml:lang="en">This property describe the directory code, which corresponds to the property cdm:resource_legal_is_about_concept_directory-code.</rdfs:comment>
        <rdfs:domain rdf:resource="&sioc;Forum"/>
    </owl:AnnotationProperty>
    


    <!-- http://lod-dk/ontologies/LOD_Epartcipation#id_celex -->

    <owl:AnnotationProperty rdf:about="&lod;id_celex">
        <rdfs:comment xml:lang="en">The property describe the id_celex, which corresponds to the property cdm:resource_legal_number_natural_celex.</rdfs:comment>
        <rdfs:domain rdf:resource="&sioc;Forum"/>
    </owl:AnnotationProperty>
    


    <!-- http://lod-dk/ontologies/LOD_Epartcipation#nationality -->

    <owl:AnnotationProperty rdf:about="&lod;nationality">
        <rdfs:label xml:lang="en">nationality</rdfs:label>
        <rdfs:comment xml:lang="en">The nationality of the user</rdfs:comment>
    </owl:AnnotationProperty>
    


    <!-- http://lod-dk/ontologies/LOD_Epartcipation#num_amendment -->

    <owl:AnnotationProperty rdf:about="&lod;num_amendment">
        <rdfs:label xml:lang="en">num_amendment</rdfs:label>
        <rdfs:comment xml:lang="en">The total number of amendments for a specific container, in considering the amendments of belonged sub-containers</rdfs:comment>
        <rdfs:domain rdf:resource="&sioc;Thread"/>
    </owl:AnnotationProperty>
    


    <!-- http://lod-dk/ontologies/LOD_Epartcipation#num_amendment_na -->

    <owl:AnnotationProperty rdf:about="&lod;num_amendment_na">
        <rdfs:label xml:lang="en">num_amendment_na</rdfs:label>
        <rdfs:comment xml:lang="en">The total number of amendments for a specific container, in considering the amendments of belonged sub-containers (&quot;na&quot; means no aggregate)</rdfs:comment>
        <rdfs:domain rdf:resource="&sioc;Thread"/>
    </owl:AnnotationProperty>
    


    <!-- http://lod-dk/ontologies/LOD_Epartcipation#num_deletion -->

    <owl:AnnotationProperty rdf:about="&lod;num_deletion">
        <rdfs:label xml:lang="en">num_deletion</rdfs:label>
        <rdfs:comment xml:lang="en">The number of deletions for a specific container, in concidering the deletion of belonged sub-containers</rdfs:comment>
        <rdfs:domain rdf:resource="&sioc;Thread"/>
    </owl:AnnotationProperty>
    


    <!-- http://lod-dk/ontologies/LOD_Epartcipation#num_deletion_na -->

    <owl:AnnotationProperty rdf:about="&lod;num_deletion_na">
        <rdfs:label xml:lang="en">num_deletion_na</rdfs:label>
        <rdfs:comment xml:lang="en">The number of deletions for a specific container, in concidering the deletion of belonged sub-containers (&quot;na&quot; means no aggregated)</rdfs:comment>
        <rdfs:domain rdf:resource="&sioc;Thread"/>
    </owl:AnnotationProperty>
    


    <!-- http://lod-dk/ontologies/LOD_Epartcipation#num_insertion -->

    <owl:AnnotationProperty rdf:about="&lod;num_insertion">
        <rdfs:label xml:lang="en">num_insertion</rdfs:label>
        <rdfs:comment xml:lang="en">The number of insertions for a specific container, in concidering the insertion of belonged sub-containers</rdfs:comment>
        <rdfs:domain rdf:resource="&sioc;Thread"/>
    </owl:AnnotationProperty>
    


    <!-- http://lod-dk/ontologies/LOD_Epartcipation#num_insertion_na -->

    <owl:AnnotationProperty rdf:about="&lod;num_insertion_na">
        <rdfs:label xml:lang="en">num_insertion_na</rdfs:label>
        <rdfs:comment xml:lang="en">The number of insertions for a specific container, in concidering the insertions of belonged sub-containers (&quot;na&quot; means no aggregated)</rdfs:comment>
        <rdfs:domain rdf:resource="&sioc;Thread"/>
    </owl:AnnotationProperty>
    


    <!-- http://lod-dk/ontologies/LOD_Epartcipation#num_items_mixed -->

    <owl:AnnotationProperty rdf:about="&lod;num_items_mixed">
        <rdfs:label xml:lang="en">num_items_mixed</rdfs:label>
        <rdfs:comment xml:lang="en">The number of neutral comments for a specific container, in concidering the comments of belonged sub-containers</rdfs:comment>
        <rdfs:domain rdf:resource="&sioc;Container"/>
    </owl:AnnotationProperty>
    


    <!-- http://lod-dk/ontologies/LOD_Epartcipation#num_items_mixed_na -->

    <owl:AnnotationProperty rdf:about="&lod;num_items_mixed_na">
        <rdfs:label xml:lang="en">num_items_mixed_na</rdfs:label>
        <rdfs:comment xml:lang="en">The number of neutral comments for a specific container, without concidering the comments of belonged sub-containers (&quot;na&quot; means no aggregated)</rdfs:comment>
        <rdfs:domain rdf:resource="&sioc;Container"/>
    </owl:AnnotationProperty>
    


    <!-- http://lod-dk/ontologies/LOD_Epartcipation#num_items_no -->

    <owl:AnnotationProperty rdf:about="&lod;num_items_no">
        <rdfs:label xml:lang="en">num_items_no </rdfs:label>
        <rdfs:comment xml:lang="en">The number of negative comments for a specific container, in concidering the comments of belonged sub-containers </rdfs:comment>
        <rdfs:domain rdf:resource="&sioc;Container"/>
    </owl:AnnotationProperty>
    


    <!-- http://lod-dk/ontologies/LOD_Epartcipation#num_items_no_na -->

    <owl:AnnotationProperty rdf:about="&lod;num_items_no_na">
        <rdfs:label xml:lang="en">num_items_no_na</rdfs:label>
        <rdfs:comment xml:lang="en">The number of negative comments for a specific container, without concidering the comments of belonged sub-containers (&quot;na&quot; means no aggregated)</rdfs:comment>
        <rdfs:domain rdf:resource="&sioc;Container"/>
    </owl:AnnotationProperty>
    


    <!-- http://lod-dk/ontologies/LOD_Epartcipation#num_items_total -->

    <owl:AnnotationProperty rdf:about="&lod;num_items_total">
        <rdfs:label xml:lang="en">num_items_total </rdfs:label>
        <rdfs:comment xml:lang="en">The number of total comments for a specific container, in concidering the comments of belonged sub-containers</rdfs:comment>
        <rdfs:domain rdf:resource="&sioc;Container"/>
    </owl:AnnotationProperty>
    


    <!-- http://lod-dk/ontologies/LOD_Epartcipation#num_items_total_na -->

    <owl:AnnotationProperty rdf:about="&lod;num_items_total_na">
        <rdfs:label xml:lang="en">num_items_total_na</rdfs:label>
        <rdfs:comment xml:lang="en">The total number of comments for a specific container, without concidering the comments of belonged sub-containers (&quot;na&quot; means no aggregated)</rdfs:comment>
        <rdfs:domain rdf:resource="&sioc;Container"/>
    </owl:AnnotationProperty>
    


    <!-- http://lod-dk/ontologies/LOD_Epartcipation#num_items_yes -->

    <owl:AnnotationProperty rdf:about="&lod;num_items_yes">
        <rdfs:label xml:lang="en">num_items_yes</rdfs:label>
        <rdfs:comment xml:lang="en">The number of positive comments for a specific container, in concidering the comments of belonged sub-containers</rdfs:comment>
        <rdfs:domain rdf:resource="&sioc;Container"/>
    </owl:AnnotationProperty>
    


    <!-- http://lod-dk/ontologies/LOD_Epartcipation#num_items_yes_na -->

    <owl:AnnotationProperty rdf:about="&lod;num_items_yes_na">
        <rdfs:label xml:lang="en">num_items_yes_na </rdfs:label>
        <rdfs:comment xml:lang="en">The number of positive comments for a specific container, without concidering the comments of belonged sub-containers (&quot;na&quot; means no aggregated)</rdfs:comment>
        <rdfs:domain rdf:resource="&sioc;Container"/>
    </owl:AnnotationProperty>
    


    <!-- http://lod-dk/ontologies/LOD_Epartcipation#num_substitution -->

    <owl:AnnotationProperty rdf:about="&lod;num_substitution">
        <rdfs:label xml:lang="en">num_substitution</rdfs:label>
        <rdfs:comment xml:lang="en">The number of substitutions for a specific container, in concidering the substitution of belonged sub-containers </rdfs:comment>
        <rdfs:domain rdf:resource="&sioc;Thread"/>
    </owl:AnnotationProperty>
    


    <!-- http://lod-dk/ontologies/LOD_Epartcipation#num_substitution_na -->

    <owl:AnnotationProperty rdf:about="&lod;num_substitution_na">
        <rdfs:label xml:lang="en">num_substitution_na</rdfs:label>
        <rdfs:comment xml:lang="en">The number of substitutions for a specific container, in concidering the substitutions of belonged sub-containers (&quot;na&quot; means no aggregated)</rdfs:comment>
        <rdfs:domain rdf:resource="&sioc;Thread"/>
    </owl:AnnotationProperty>
    


    <!-- http://lod-dk/ontologies/LOD_Epartcipation#password -->

    <owl:AnnotationProperty rdf:about="&lod;password">
        <rdfs:domain rdf:resource="&sioc;UserAccount"/>
    </owl:AnnotationProperty>
    


    <!-- http://lod-dk/ontologies/LOD_Epartcipation#procedure_code -->

    <owl:AnnotationProperty rdf:about="&lod;procedure_code">
        <rdfs:comment xml:lang="en">The property correspond to cdm:procedure_code_interinstitutional_reference_procedure</rdfs:comment>
        <rdfs:domain rdf:resource="&sioc;Forum"/>
    </owl:AnnotationProperty>
    


    <!-- http://lod-dk/ontologies/LOD_Epartcipation#procedure_number -->

    <owl:AnnotationProperty rdf:about="&lod;procedure_number">
        <rdfs:comment xml:lang="en">The property corresponds at: cdm:procedure_code_interinstitutional_number_procedure</rdfs:comment>
        <rdfs:domain rdf:resource="&sioc;Forum"/>
    </owl:AnnotationProperty>
    


    <!-- http://lod-dk/ontologies/LOD_Epartcipation#procedure_type -->

    <owl:AnnotationProperty rdf:about="&lod;procedure_type">
        <rdfs:label xml:lang="en">procedure_type</rdfs:label>
        <rdfs:comment xml:lang="en">The procedure_type property corresponds to: cdm:procedure_code_interinstitutional_has_type_concept_type_procedure_code_interinstitutional</rdfs:comment>
    </owl:AnnotationProperty>
    


    <!-- http://lod-dk/ontologies/LOD_Epartcipation#procedure_year -->

    <owl:AnnotationProperty rdf:about="&lod;procedure_year">
        <rdfs:label xml:lang="en">procedure_year</rdfs:label>
        <rdfs:comment xml:lang="en">The property procedure_year correspond at: cdm:procedure_code_interinstitutional_year_procedure</rdfs:comment>
        <rdfs:domain rdf:resource="&sioc;Forum"/>
    </owl:AnnotationProperty>
    


    <!-- http://lod-dk/ontologies/LOD_Epartcipation#reputation -->

    <owl:AnnotationProperty rdf:about="&lod;reputation">
        <rdfs:label xml:lang="en">reputation</rdfs:label>
        <rdfs:comment xml:lang="en">The reputation of user is computed according to specifics function and in considering a specific events</rdfs:comment>
        <rdfs:domain rdf:resource="&sioc;UserAccount"/>
    </owl:AnnotationProperty>
    


    <!-- http://lod-dk/ontologies/LOD_Epartcipation#subject -->

    <owl:AnnotationProperty rdf:about="&lod;subject">
        <rdfs:label xml:lang="en">subject</rdfs:label>
        <rdfs:comment xml:lang="en">The subject of the act (sub-part of the title)</rdfs:comment>
        <rdfs:domain rdf:resource="&sioc;Forum"/>
    </owl:AnnotationProperty>
    


    <!-- http://lod-dk/ontologies/LOD_Epartcipation#title -->

    <owl:AnnotationProperty rdf:about="&lod;title">
        <rdfs:label xml:lang="en">title</rdfs:label>
        <rdfs:comment xml:lang="en">The title of the act, i.e. legal resource</rdfs:comment>
        <rdfs:domain rdf:resource="&sioc;Forum"/>
    </owl:AnnotationProperty>
    


    <!-- http://lod-dk/ontologies/LOD_Epartcipation#token_date -->

    <owl:AnnotationProperty rdf:about="&lod;token_date">
        <rdfs:comment xml:lang="en">The propery correspond to the deadline given to the user to modify his passeword. </rdfs:comment>
        <rdfs:domain rdf:resource="&sioc;UserAccount"/>
    </owl:AnnotationProperty>
    


    <!-- http://lod-dk/ontologies/LOD_Epartcipation#token_id -->

    <owl:AnnotationProperty rdf:about="&lod;token_id">
        <rdfs:comment xml:lang="en">The property is a randome number given to the user, in order to modify his passeword. This property is crypted.</rdfs:comment>
        <rdfs:domain rdf:resource="&sioc;UserAccount"/>
    </owl:AnnotationProperty>
    


    <!-- http://lod-dk/ontologies/LOD_Epartcipation#topic -->

    <owl:AnnotationProperty rdf:about="&lod;topic">
        <rdfs:label xml:lang="en">topic</rdfs:label>
        <rdfs:comment xml:lang="en">The property corresponds to cdm:work_is_about_concept_eurovoc. 
There existe in cdm another property cdm:is_about_*, but we consider only the eurovoc concept.</rdfs:comment>
    </owl:AnnotationProperty>
    


    <!-- 
    ///////////////////////////////////////////////////////////////////////////////////////
    //
    // Datatypes
    //
    ///////////////////////////////////////////////////////////////////////////////////////
     -->

    


    <!-- http://www.w3.org/1999/02/22-rdf-syntax-ns#LangString -->

    <rdfs:Datatype rdf:about="&rdf;LangString"/>
    


    <!-- http://www.w3.org/1999/02/22-rdf-syntax-ns#Literal -->

    <rdfs:Datatype rdf:about="&rdf;Literal"/>
    


    <!-- http://www.w3.org/2001/XMLSchema#gYear -->

    <rdfs:Datatype rdf:about="&xsd;gYear"/>
    


    <!-- 
    ///////////////////////////////////////////////////////////////////////////////////////
    //
    // Object Properties
    //
    ///////////////////////////////////////////////////////////////////////////////////////
     -->

    


    <!-- http://lod-dk/ontologies/LOD_Epartcipation#contained -->

    <owl:ObjectProperty rdf:about="&lod;contained">
        <rdfs:label xml:lang="en">contained</rdfs:label>
        <rdfs:comment xml:lang="en">this property links the amendment to the post, if the amendment contains post</rdfs:comment>
        <rdfs:domain rdf:resource="&prv;ContentAmendment"/>
        <rdfs:range rdf:resource="&sioc;Post"/>
    </owl:ObjectProperty>
    


    <!-- http://lod-dk/ontologies/LOD_Epartcipation#contains -->

    <owl:ObjectProperty rdf:about="&lod;contains">
        <rdfs:label xml:lang="en">contains</rdfs:label>
        <rdfs:comment xml:lang="en">this property links the post to the amendment, if the post contains amendment</rdfs:comment>
        <owl:inverseOf rdf:resource="&lod;contained"/>
        <rdfs:range rdf:resource="&prv;ContentAmendment"/>
        <rdfs:domain rdf:resource="&sioc;Post"/>
    </owl:ObjectProperty>
    


    <!-- http://lod-dk/ontologies/LOD_Epartcipation#nationality -->

    <owl:ObjectProperty rdf:about="&lod;nationality">
        <rdfs:label xml:lang="en">nationality</rdfs:label>
        <rdfs:comment xml:lang="en">The nationality of the user</rdfs:comment>
        <rdfs:domain rdf:resource="&sioc;UserAccount"/>
        <rdfs:range rdf:resource="http://schema.org#country"/>
    </owl:ObjectProperty>
    


    <!-- http://lod-dk/ontologies/LOD_Epartcipation#procedure_type -->

    <owl:ObjectProperty rdf:about="&lod;procedure_type">
        <rdfs:label xml:lang="en">procedure_type</rdfs:label>
        <rdfs:comment xml:lang="en">The procedure_type property corresponds to: cdm:procedure_code_interinstitutional_has_type_concept_type_procedure_code_interinstitutional</rdfs:comment>
        <rdfs:range rdf:resource="&cdm;concept_type_procedure_code_interinstitutional"/>
        <rdfs:domain rdf:resource="&sioc;Forum"/>
    </owl:ObjectProperty>
    


    <!-- http://lod-dk/ontologies/LOD_Epartcipation#topic -->

    <owl:ObjectProperty rdf:about="&lod;topic">
        <rdfs:label xml:lang="en">topic</rdfs:label>
        <rdfs:comment xml:lang="en">The property corresponds to cdm:work_is_about_concept_eurovoc. 
There existe in cdm another property cdm:is_about_*, but we consider only the eurovoc concept.</rdfs:comment>
        <rdfs:range rdf:resource="&cdm;concept"/>
        <rdfs:domain rdf:resource="&sioc;Forum"/>
    </owl:ObjectProperty>
    


    <!-- 
    ///////////////////////////////////////////////////////////////////////////////////////
    //
    // Data properties
    //
    ///////////////////////////////////////////////////////////////////////////////////////
     -->

    


    <!-- http://lod-dk/ontologies/LOD_Epartcipation#amended_at -->

    <owl:DatatypeProperty rdf:about="&lod;amended_at">
        <rdfs:comment>This property is used when the user edite his comment and gives modification. The timesteemp of this modification  is descriped in this property. Outherwise, this property is empty. </rdfs:comment>
        <rdfs:domain rdf:resource="&sioc;Post"/>
        <rdfs:range rdf:resource="&rdfs;Literal"/>
    </owl:DatatypeProperty>
    


    <!-- http://lod-dk/ontologies/LOD_Epartcipation#created_at -->

    <owl:DatatypeProperty rdf:about="&lod;created_at">
        <rdfs:comment>This property describe the date of the creation of act, which correspond to the property cdm:cdm:work_date_document.</rdfs:comment>
        <rdfs:domain rdf:resource="&sioc;Forum"/>
        <rdfs:range rdf:resource="&rdfs;Literal"/>
    </owl:DatatypeProperty>
    


    <!-- http://lod-dk/ontologies/LOD_Epartcipation#directory_code -->

    <owl:DatatypeProperty rdf:about="&lod;directory_code">
        <rdfs:comment xml:lang="en">This property describe the directory code, which corresponds to the property cdm:resource_legal_is_about_concept_directory-code.</rdfs:comment>
        <rdfs:range rdf:resource="&rdfs;Literal"/>
    </owl:DatatypeProperty>
    


    <!-- http://lod-dk/ontologies/LOD_Epartcipation#id_celex -->

    <owl:DatatypeProperty rdf:about="&lod;id_celex">
        <rdfs:comment xml:lang="en">The property describe the id_celex, which corresponds to the property cdm:resource_legal_number_natural_celex.</rdfs:comment>
        <rdfs:range rdf:resource="&rdfs;Literal"/>
    </owl:DatatypeProperty>
    


    <!-- http://lod-dk/ontologies/LOD_Epartcipation#num_amendment -->

    <owl:DatatypeProperty rdf:about="&lod;num_amendment">
        <rdfs:label xml:lang="en">num_amendment</rdfs:label>
        <rdfs:comment xml:lang="en">The total number of amendments for a specific container, in considering the amendments of belonged sub-containers</rdfs:comment>
        <rdfs:range rdf:resource="&xsd;nonNegativeInteger"/>
    </owl:DatatypeProperty>
    


    <!-- http://lod-dk/ontologies/LOD_Epartcipation#num_amendment_na -->

    <owl:DatatypeProperty rdf:about="&lod;num_amendment_na">
        <rdfs:label xml:lang="en">num_amendment_na</rdfs:label>
        <rdfs:comment xml:lang="en">The total number of amendments for a specific container, in considering the amendments of belonged sub-containers (&quot;na&quot; means no aggregate)</rdfs:comment>
        <rdfs:range rdf:resource="&xsd;nonNegativeInteger"/>
    </owl:DatatypeProperty>
    


    <!-- http://lod-dk/ontologies/LOD_Epartcipation#num_deletion -->

    <owl:DatatypeProperty rdf:about="&lod;num_deletion">
        <rdfs:label xml:lang="en">num_deletion</rdfs:label>
        <rdfs:comment xml:lang="en">The number of deletions for a specific container, in concidering the deletion of belonged sub-containers</rdfs:comment>
        <rdfs:range rdf:resource="&xsd;nonNegativeInteger"/>
    </owl:DatatypeProperty>
    


    <!-- http://lod-dk/ontologies/LOD_Epartcipation#num_deletion_na -->

    <owl:DatatypeProperty rdf:about="&lod;num_deletion_na">
        <rdfs:label xml:lang="en">num_deletion_na</rdfs:label>
        <rdfs:comment xml:lang="en">The number of deletions for a specific container, in concidering the deletion of belonged sub-containers (&quot;na&quot; means no aggregated)</rdfs:comment>
        <rdfs:range rdf:resource="&xsd;nonNegativeInteger"/>
    </owl:DatatypeProperty>
    


    <!-- http://lod-dk/ontologies/LOD_Epartcipation#num_dislike -->

    <owl:DatatypeProperty rdf:about="&lod;num_dislike">
        <rdfs:label xml:lang="en">num_dislike</rdfs:label>
        <rdfs:comment xml:lang="en">The num_dislike of the post, which given by the authers posts. These posts give only the note</rdfs:comment>
        <rdfs:domain rdf:resource="&sioc;Post"/>
        <rdfs:range rdf:resource="&xsd;nonNegativeInteger"/>
    </owl:DatatypeProperty>
    


    <!-- http://lod-dk/ontologies/LOD_Epartcipation#num_insertion -->

    <owl:DatatypeProperty rdf:about="&lod;num_insertion">
        <rdfs:label xml:lang="en">num_insertion</rdfs:label>
        <rdfs:comment xml:lang="en">The number of insertions for a specific container, in concidering the insertion of belonged sub-containers</rdfs:comment>
        <rdfs:range rdf:resource="&xsd;nonNegativeInteger"/>
    </owl:DatatypeProperty>
    


    <!-- http://lod-dk/ontologies/LOD_Epartcipation#num_insertion_na -->

    <owl:DatatypeProperty rdf:about="&lod;num_insertion_na">
        <rdfs:label xml:lang="en">num_insertion_na</rdfs:label>
        <rdfs:comment xml:lang="en">The number of insertions for a specific container, in concidering the insertions of belonged sub-containers (&quot;na&quot; means no aggregated)</rdfs:comment>
        <rdfs:range rdf:resource="&xsd;nonNegativeInteger"/>
    </owl:DatatypeProperty>
    


    <!-- http://lod-dk/ontologies/LOD_Epartcipation#num_items_mixed -->

    <owl:DatatypeProperty rdf:about="&lod;num_items_mixed">
        <rdfs:label xml:lang="en">num_items_mixed</rdfs:label>
        <rdfs:comment xml:lang="en">The number of neutral comments for a specific container, in concidering the comments of belonged sub-containers</rdfs:comment>
        <rdfs:range rdf:resource="&xsd;nonNegativeInteger"/>
    </owl:DatatypeProperty>
    


    <!-- http://lod-dk/ontologies/LOD_Epartcipation#num_items_mixed_na -->

    <owl:DatatypeProperty rdf:about="&lod;num_items_mixed_na">
        <rdfs:label xml:lang="en">num_items_mixed_na</rdfs:label>
        <rdfs:comment xml:lang="en">The number of neutral comments for a specific container, without concidering the comments of belonged sub-containers (&quot;na&quot; means no aggregated)</rdfs:comment>
        <rdfs:range rdf:resource="&xsd;nonNegativeInteger"/>
    </owl:DatatypeProperty>
    


    <!-- http://lod-dk/ontologies/LOD_Epartcipation#num_items_no -->

    <owl:DatatypeProperty rdf:about="&lod;num_items_no">
        <rdfs:label xml:lang="en">num_items_no </rdfs:label>
        <rdfs:comment xml:lang="en">The number of negative comments for a specific container, in concidering the comments of belonged sub-containers </rdfs:comment>
        <rdfs:range rdf:resource="&xsd;nonNegativeInteger"/>
    </owl:DatatypeProperty>
    


    <!-- http://lod-dk/ontologies/LOD_Epartcipation#num_items_no_na -->

    <owl:DatatypeProperty rdf:about="&lod;num_items_no_na">
        <rdfs:label xml:lang="en">num_items_no_na</rdfs:label>
        <rdfs:comment xml:lang="en">The number of negative comments for a specific container, without concidering the comments of belonged sub-containers (&quot;na&quot; means no aggregated)</rdfs:comment>
        <rdfs:range rdf:resource="&xsd;nonNegativeInteger"/>
    </owl:DatatypeProperty>
    


    <!-- http://lod-dk/ontologies/LOD_Epartcipation#num_items_total -->

    <owl:DatatypeProperty rdf:about="&lod;num_items_total">
        <rdfs:label xml:lang="en">num_items_total </rdfs:label>
        <rdfs:comment xml:lang="en">The number of total comments for a specific container, in concidering the comments of belonged sub-containers</rdfs:comment>
        <rdfs:range rdf:resource="&xsd;nonNegativeInteger"/>
    </owl:DatatypeProperty>
    


    <!-- http://lod-dk/ontologies/LOD_Epartcipation#num_items_total_na -->

    <owl:DatatypeProperty rdf:about="&lod;num_items_total_na">
        <rdfs:label xml:lang="en">num_items_total_na</rdfs:label>
        <rdfs:comment xml:lang="en">The total number of comments for a specific container, without concidering the comments of belonged sub-containers (&quot;na&quot; means no aggregated)</rdfs:comment>
        <rdfs:range rdf:resource="&xsd;nonNegativeInteger"/>
    </owl:DatatypeProperty>
    


    <!-- http://lod-dk/ontologies/LOD_Epartcipation#num_items_yes -->

    <owl:DatatypeProperty rdf:about="&lod;num_items_yes">
        <rdfs:label xml:lang="en">num_items_yes</rdfs:label>
        <rdfs:comment xml:lang="en">The number of positive comments for a specific container, in concidering the comments of belonged sub-containers</rdfs:comment>
        <rdfs:range rdf:resource="&xsd;nonNegativeInteger"/>
    </owl:DatatypeProperty>
    


    <!-- http://lod-dk/ontologies/LOD_Epartcipation#num_items_yes_na -->

    <owl:DatatypeProperty rdf:about="&lod;num_items_yes_na">
        <rdfs:label xml:lang="en">num_items_yes_na </rdfs:label>
        <rdfs:comment xml:lang="en">The number of positive comments for a specific container, without concidering the comments of belonged sub-containers (&quot;na&quot; means no aggregated)</rdfs:comment>
        <rdfs:range rdf:resource="&xsd;nonNegativeInteger"/>
    </owl:DatatypeProperty>
    


    <!-- http://lod-dk/ontologies/LOD_Epartcipation#num_like -->

    <owl:DatatypeProperty rdf:about="&lod;num_like">
        <rdfs:label xml:lang="en">num_like</rdfs:label>
        <rdfs:comment xml:lang="en">The num_like of the post, which given by the authers posts. These posts give only the note</rdfs:comment>
        <rdfs:domain rdf:resource="&sioc;Post"/>
        <rdfs:range rdf:resource="&xsd;nonNegativeInteger"/>
    </owl:DatatypeProperty>
    


    <!-- http://lod-dk/ontologies/LOD_Epartcipation#num_substitution -->

    <owl:DatatypeProperty rdf:about="&lod;num_substitution">
        <rdfs:label xml:lang="en">num_substitution</rdfs:label>
        <rdfs:comment xml:lang="en">The number of substitutions for a specific container, in concidering the substitution of belonged sub-containers </rdfs:comment>
        <rdfs:range rdf:resource="&xsd;nonNegativeInteger"/>
    </owl:DatatypeProperty>
    


    <!-- http://lod-dk/ontologies/LOD_Epartcipation#num_substitution_na -->

    <owl:DatatypeProperty rdf:about="&lod;num_substitution_na">
        <rdfs:label xml:lang="en">num_substitution_na</rdfs:label>
        <rdfs:comment xml:lang="en">The number of substitutions for a specific container, in concidering the substitutions of belonged sub-containers (&quot;na&quot; means no aggregated)</rdfs:comment>
        <rdfs:range rdf:resource="&xsd;nonNegativeInteger"/>
    </owl:DatatypeProperty>
    


    <!-- http://lod-dk/ontologies/LOD_Epartcipation#password -->

    <owl:DatatypeProperty rdf:about="&lod;password">
        <rdfs:range rdf:resource="&rdfs;Literal"/>
    </owl:DatatypeProperty>
    


    <!-- http://lod-dk/ontologies/LOD_Epartcipation#procedure_code -->

    <owl:DatatypeProperty rdf:about="&lod;procedure_code">
        <rdfs:comment xml:lang="en">The property correspond to cdm:procedure_code_interinstitutional_reference_procedure</rdfs:comment>
        <rdfs:range rdf:resource="&rdfs;Literal"/>
    </owl:DatatypeProperty>
    


    <!-- http://lod-dk/ontologies/LOD_Epartcipation#procedure_number -->

    <owl:DatatypeProperty rdf:about="&lod;procedure_number">
        <rdfs:comment xml:lang="en">The property corresponds at: cdm:procedure_code_interinstitutional_number_procedure</rdfs:comment>
        <rdfs:range rdf:resource="&rdfs;Literal"/>
    </owl:DatatypeProperty>
    


    <!-- http://lod-dk/ontologies/LOD_Epartcipation#procedure_year -->

    <owl:DatatypeProperty rdf:about="&lod;procedure_year">
        <rdfs:label xml:lang="en">procedure_year</rdfs:label>
        <rdfs:comment xml:lang="en">The property procedure_year correspond at: cdm:procedure_code_interinstitutional_year_procedure</rdfs:comment>
        <rdfs:range rdf:resource="&xsd;gYear"/>
    </owl:DatatypeProperty>
    


    <!-- http://lod-dk/ontologies/LOD_Epartcipation#reputation -->

    <owl:DatatypeProperty rdf:about="&lod;reputation">
        <rdfs:label xml:lang="en">reputation</rdfs:label>
        <rdfs:comment xml:lang="en">The reputation of user is computed according to specifics function and in considering a specific events</rdfs:comment>
        <rdfs:range rdf:resource="&xsd;integer"/>
    </owl:DatatypeProperty>
    


    <!-- http://lod-dk/ontologies/LOD_Epartcipation#subject -->

    <owl:DatatypeProperty rdf:about="&lod;subject">
        <rdfs:label xml:lang="en">subject</rdfs:label>
        <rdfs:comment xml:lang="en">The subject of the act (sub-part of the title)</rdfs:comment>
        <rdfs:range rdf:resource="&rdf;LangString"/>
    </owl:DatatypeProperty>
    


    <!-- http://lod-dk/ontologies/LOD_Epartcipation#tag -->

    <owl:DatatypeProperty rdf:about="&lod;tag">
        <rdfs:label xml:lang="en">tag</rdfs:label>
        <rdfs:comment xml:lang="en">The tag of the post, which corresponds to the thematics of the comments</rdfs:comment>
        <rdfs:domain rdf:resource="&sioc;Post"/>
        <rdfs:range rdf:resource="&rdf;LangString"/>
    </owl:DatatypeProperty>
    


    <!-- http://lod-dk/ontologies/LOD_Epartcipation#title -->

    <owl:DatatypeProperty rdf:about="&lod;title">
        <rdfs:label xml:lang="en">title</rdfs:label>
        <rdfs:comment xml:lang="en">The title of the act, i.e. legal resource</rdfs:comment>
        <rdfs:range rdf:resource="&rdf;LangString"/>
    </owl:DatatypeProperty>
    


    <!-- http://lod-dk/ontologies/LOD_Epartcipation#token_date -->

    <owl:DatatypeProperty rdf:about="&lod;token_date">
        <rdfs:comment xml:lang="en">The propery correspond to the deadline given to the user to modify his passeword. </rdfs:comment>
        <rdfs:range rdf:resource="&rdfs;Literal"/>
    </owl:DatatypeProperty>
    


    <!-- http://lod-dk/ontologies/LOD_Epartcipation#token_id -->

    <owl:DatatypeProperty rdf:about="&lod;token_id">
        <rdfs:comment xml:lang="en">The property is a randome number given to the user, in order to modify his passeword. This property is crypted.</rdfs:comment>
        <rdfs:range rdf:resource="&rdfs;Literal"/>
    </owl:DatatypeProperty>
    


    <!-- 
    ///////////////////////////////////////////////////////////////////////////////////////
    //
    // Classes
    //
    ///////////////////////////////////////////////////////////////////////////////////////
     -->

    


    <!-- http://lod-dk/ontologies/ProvisionModel#ContentAmendment -->

    <owl:Class rdf:about="&prv;ContentAmendment"/>
    


    <!-- http://publications.europa.eu/ontology/cdm#concept -->

    <owl:Class rdf:about="&cdm;concept"/>
    


    <!-- http://publications.europa.eu/ontology/cdm#concept_type_procedure_code_interinstitutional -->

    <owl:Class rdf:about="&cdm;concept_type_procedure_code_interinstitutional"/>
    


    <!-- http://rdfs.org/sioc/ns#Container -->

    <owl:Class rdf:about="&sioc;Container"/>
    


    <!-- http://rdfs.org/sioc/ns#Forum -->

    <owl:Class rdf:about="&sioc;Forum"/>
    


    <!-- http://rdfs.org/sioc/ns#Post -->

    <owl:Class rdf:about="&sioc;Post"/>
    


    <!-- http://rdfs.org/sioc/ns#Thread -->

    <owl:Class rdf:about="&sioc;Thread"/>
    


    <!-- http://rdfs.org/sioc/ns#UserAccount -->

    <owl:Class rdf:about="&sioc;UserAccount"/>
    


    <!-- http://schema.org#country -->

    <owl:Class rdf:about="http://schema.org#country"/>
    


    <!-- 
    ///////////////////////////////////////////////////////////////////////////////////////
    //
    // Individuals
    //
    ///////////////////////////////////////////////////////////////////////////////////////
     -->

    


    <!-- http://lod-dk/ontologies/LOD_Eparticipation# -->

    <owl:Thing rdf:about="http://lod-dk/ontologies/LOD_Eparticipation#">
        <rdf:type rdf:resource="&owl;NamedIndividual"/>
    </owl:Thing>
    


    <!-- 
    ///////////////////////////////////////////////////////////////////////////////////////
    //
    // Annotations
    //
    ///////////////////////////////////////////////////////////////////////////////////////
     -->

    <rdf:Description rdf:about="http://rdfs.org/sioc/spec">
        <rdfs:label>SIOC Core Ontology Specification</rdfs:label>
    </rdf:Description>
</rdf:RDF>



<!-- Generated by the OWL API (version 3.4.2) http://owlapi.sourceforge.net -->

